out/InductNatExample.v
@@ -6,15 +6,15 @@ Inductive Natural: Set := ZeroN: Natural | Suc: (Natural -> Natural).
 Load IntNatExample. 
 Definition one := Suc ZeroN. 
 Definition two := Suc one. 
-Definition toInt_unrefined (n: { n : Natural | True }): { v : BinNums.Z | v>=0 }. 
+Definition toInt_unrefined (n: { n : Natural | True }): { VV : BinNums.Z | (VV>=(0)) }. 
 Proof.
   destruct n as [n np ]. 
   induction n as [| n IHn ]. 
-    { smt_now unshelve refine (injectionCast BinNums.Z (fun v: BinNums.Z => v>=0) (0) _). }
-    { smt_now unshelve refine (injectionCast BinNums.Z (fun v: BinNums.Z => v>=0) (1+(` (IHn))) _). }
+    { smt_now unshelve refine (injectionCast BinNums.Z (fun VV: BinNums.Z => (VV>=(0))) (0) _). }
+    { smt_now unshelve refine (injectionCast BinNums.Z (fun VV: BinNums.Z => (VV>=(0))) ((1)+(` (IHn))) _). }
 Defined.
 
-Definition toInt (n: { n : Natural | True }): { v : BinNums.Z | (` (toInt_unrefined n))=v } .
+Definition toInt (n: { n : Natural | True }): { VV : BinNums.Z | ((` (toInt_unrefined n))=(VV)) } .
 Proof.
   destruct n as [n np ]. 
   exact (exist (` (toInt_unrefined (injectionCast Natural (fun n: Natural => True) (n) _))) eq_refl). 
@@ -28,7 +28,7 @@ Proof.
     { smt_now unshelve refine (injectionCast Natural (fun VV: Natural => True) (Suc (` (IHm))) _). }
 Defined.
 
-Definition add (m: { m : Natural | True }) (n: { n : Natural | True }): { VV : Natural | (` (add_unrefined m n))=VV } .
+Definition add (m: { m : Natural | True }) (n: { n : Natural | True }): { VV : Natural | ((` (add_unrefined m n))=(VV)) } .
 Proof.
   destruct m as [m mp ].  destruct n as [n np ]. 
   exact (exist (` (add_unrefined (injectionCast Natural (fun m: Natural => True) (m) _) (injectionCast Natural (fun n: Natural => True) (n) _))) eq_refl). 
@@ -39,17 +39,99 @@ Proof.
   destruct m as [m mp ].  destruct n as [n np ]. 
   induction m as [| m IHm ]. 
     { smt_now unshelve refine (injectionCast Natural (fun VV: Natural => True) (ZeroN) _). }
-    { smt_now unshelve refine (subsumptionCast Natural (fun VV: Natural => (` (add_unrefined (injectionCast Natural (fun n: Natural => True) (n) _) IHm))=VV) (fun VV: Natural => True) _ (add (injectionCast Natural (fun m: Natural => True) (n) _) IHm)). }
+    { smt_now unshelve refine (subsumptionCast Natural (fun VV: Natural => ((` (add_unrefined (injectionCast Natural (fun n: Natural => True) (n) _) IHm))=(VV))) (fun VV: Natural => True) _ (add (injectionCast Natural (fun m: Natural => True) (n) _) IHm)). }
 Defined.
 
-Definition mult (m: { m : Natural | True }) (n: { n : Natural | True }): { VV : Natural | (` (mult_unrefined m n))=VV } .
+Definition mult (m: { m : Natural | True }) (n: { n : Natural | True }): { VV : Natural | ((` (mult_unrefined m n))=(VV)) } .
 Proof.
   destruct m as [m mp ].  destruct n as [n np ]. 
   exact (exist (` (mult_unrefined (injectionCast Natural (fun m: Natural => True) (m) _) (injectionCast Natural (fun n: Natural => True) (n) _))) eq_refl). 
 Defined.
 
+Definition eqN_unrefined (m: { m : Natural | True }) (n: { n : Natural | True }): { r : Prop | (r=((` (m))=(` (n)))) }. 
+Proof.
+  destruct m as [m mp ].  destruct n as [n np ]. 
+  induction m as [| m IHm ]. 
+    { destruct n as [ | lq_anf7205759403792798519 ]. smt_now unshelve refine (injectionCast Prop (fun r: Prop => (r=((` (m))=(` (n))))) (True) _). smt_now unshelve refine (injectionCast Prop (fun r: Prop => (r=((` (m))=(` (n))))) (False) _). }
+    { destruct n as [ | n ]. smt_now unshelve refine (injectionCast Prop (fun r: Prop => (r=((` (m))=(` (n))))) (False) _). smt_now unshelve refine (IHm). }
+Defined.
+
+Definition eqN (m: { m : Natural | True }) (n: { n : Natural | True }): { r : Prop | ((` (eqN_unrefined m n))=(r)) } .
+Proof.
+  destruct m as [m mp ].  destruct n as [n np ]. 
+  exact (exist (` (eqN_unrefined (injectionCast Natural (fun m: Natural => True) (m) _) (injectionCast Natural (fun n: Natural => True) (n) _))) eq_refl). 
+Defined.
+
+Definition geqN_unrefined (m: { m : Natural | True }) (n: { n : Natural | True }): { p : Prop | (p=((` (toInt m))>=(` (toInt n)))) }. 
+Proof.
+  destruct m as [m mp ].  destruct n as [n np ]. 
+  induction m as [| m IHm ]. 
+    { smt_now unshelve refine (injectionCast Prop (fun p: Prop => (p=((` (toInt m))>=(` (toInt (injectionCast Natural (fun n: Natural => True) (n) _)))))) (True) _). }
+    { destruct m as [ | m ]. destruct n as [ | ds_d1ed ]. destruct () as [ ]. smt_now unshelve refine (injectionCast Prop (fun p: Prop => (p=((` (toInt m))>=(` (toInt (injectionCast Natural (fun n: Natural => True) (n) _)))))) (False) _). destruct n as [ | n ]. destruct () as [ ]. smt_now unshelve refine (IHm). }
+Defined.
+
+Definition geqN (m: { m : Natural | True }) (n: { n : Natural | True }): { p : Prop | ((` (geqN_unrefined m n))=(p)) } .
+Proof.
+  destruct m as [m mp ].  destruct n as [n np ]. 
+  exact (exist (` (geqN_unrefined (injectionCast Natural (fun m: Natural => True) (m) _) (injectionCast Natural (fun n: Natural => True) (n) _))) eq_refl). 
+Defined.
+
+Definition leqN_unrefined (m: { m : Natural | True }) (n: { n : Natural | True }): { p : Prop | (p=((` (toInt m))<=(` (toInt n)))) }. 
+Proof.
+  destruct m as [m mp ].  destruct n as [n np ]. 
+  
+    { smt_now unshelve refine (subsumptionCast Prop (fun p: Prop => ((` (geqN_unrefined (injectionCast Natural (fun n: Natural => True) (n) _) (injectionCast Natural (fun m: Natural => True) (m) _)))=(p))) (fun p: Prop => (p=((` (toInt m))<=(` (toInt (injectionCast Natural (fun n: Natural => True) (n) _)))))) _ (geqN (injectionCast Natural (fun m: Natural => True) (n) _) (injectionCast Natural (fun n: Natural => True) (m) _))). }
+Defined.
+
+Definition leqN (m: { m : Natural | True }) (n: { n : Natural | True }): { p : Prop | ((` (leqN_unrefined m n))=(p)) } .
+Proof.
+  destruct m as [m mp ].  destruct n as [n np ]. 
+  exact (exist (` (leqN_unrefined (injectionCast Natural (fun m: Natural => True) (m) _) (injectionCast Natural (fun n: Natural => True) (n) _))) eq_refl). 
+Defined.
+
+Definition geN_unrefined (m: { m : Natural | True }) (n: { n : Natural | True }): { p : Prop | p->geqN m n /\ (p=((` (toInt m))>(` (toInt n)))) }. 
+Proof.
+  destruct m as [m mp ].  destruct n as [n np ]. 
+  induction m as [| ds_d1e7 IHds_d1e7 ]. 
+    { smt_now unshelve refine (injectionCast Prop (fun p: Prop => p->geqN (injectionCast Natural (fun m: Natural => True) (m) _) (injectionCast Natural (fun n: Natural => True) (n) _) /\ (p=((` (toInt m))>(` (toInt (injectionCast Natural (fun n: Natural => True) (n) _)))))) (False) _). }
+    { destruct n as [ | n ]. smt_now unshelve refine (injectionCast Prop (fun p: Prop => p->geqN (injectionCast Natural (fun m: Natural => True) (m) _) (injectionCast Natural (fun n: Natural => True) (n) _) /\ (p=((` (toInt m))>(` (toInt (injectionCast Natural (fun n: Natural => True) (n) _)))))) (True) _). smt_now unshelve refine (IHds_d1e7). }
+Defined.
+
+Definition geN (m: { m : Natural | True }) (n: { n : Natural | True }): { p : Prop | ((` (geN_unrefined m n))=(p)) } .
+Proof.
+  destruct m as [m mp ].  destruct n as [n np ]. 
+  exact (exist (` (geN_unrefined (injectionCast Natural (fun m: Natural => True) (m) _) (injectionCast Natural (fun n: Natural => True) (n) _))) eq_refl). 
+Defined.
+
+Definition leN_unrefined (m: { m : Natural | True }) (n: { n : Natural | True }): { p : Prop | (p=((` (toInt m))<(` (toInt n)))) }. 
+Proof.
+  destruct m as [m mp ].  destruct n as [n np ]. 
+  
+    { smt_now unshelve refine (subsumptionCast Prop (fun p: Prop => ((` (geN_unrefined (injectionCast Natural (fun n: Natural => True) (n) _) (injectionCast Natural (fun m: Natural => True) (m) _)))=(p))) (fun p: Prop => (p=((` (toInt m))<(` (toInt (injectionCast Natural (fun n: Natural => True) (n) _)))))) _ (geN (injectionCast Natural (fun m: Natural => True) (n) _) (injectionCast Natural (fun n: Natural => True) (m) _))). }
+Defined.
+
+Definition leN (m: { m : Natural | True }) (n: { n : Natural | True }): { p : Prop | ((` (leN_unrefined m n))=(p)) } .
+Proof.
+  destruct m as [m mp ].  destruct n as [n np ]. 
+  exact (exist (` (leN_unrefined (injectionCast Natural (fun m: Natural => True) (m) _) (injectionCast Natural (fun n: Natural => True) (n) _))) eq_refl). 
+Defined.
+
+Definition subt_unrefined (m: { m : Natural | True }) (n: { n : Natural | geqN m n }): { o : Natural | (((` (n))<>(ZeroN))=((` (toInt (injectionCast Natural (fun n: Natural => True) (o) I)))<(` (toInt m)))) }. 
+Proof.
+  destruct m as [m mp ].  destruct n as [n np ]. 
+  induction m as [| m IHm ]. 
+    { destruct n as [ | lq_anf7205759403792798680 ]. smt_now unshelve refine (injectionCast Natural (fun o: Natural => (((` (n))<>(ZeroN))=((` (toInt (injectionCast Natural (fun n: Natural => True) (o) I)))<(` (toInt m))))) (ZeroN) _). destruct () as [ ]. }
+    { destruct n as [ | n ]. smt_now unshelve refine (injectionCast Natural (fun o: Natural => (((` (n))<>(ZeroN))=((` (toInt (injectionCast Natural (fun n: Natural => True) (o) I)))<(` (toInt m))))) (Suc m) _). smt_now unshelve refine (IHm). }
+Defined.
+
+Definition subt (m: { m : Natural | True }) (n: { n : Natural | geqN m n }): { o : Natural | ((` (subt_unrefined m n))=(o)) } .
+Proof.
+  destruct m as [m mp ].  destruct n as [n np ]. 
+  exact (exist (` (subt_unrefined (injectionCast Natural (fun m: Natural => True) (m) _) (injectionCast Natural (fun n: Natural => geqN m n) (n) _))) eq_refl). 
+Defined.
+
 Definition add_zero_l_spec: Prop. 
-Proof. now unshelve refine (forall (n:{n: Natural| True}), (` (add (injectionCast Natural (fun m: Natural => True) (ZeroN) _) n))=(` (n))). .
+Proof. smt_now unshelve refine (forall (n:{n: Natural| True}), ((` (add (injectionCast Natural (fun m: Natural => True) (ZeroN) _) n))=(` (n)))). 
 Defined.
 Theorem add_zero_l: add_zero_l_spec.
 Proof.
@@ -60,7 +142,7 @@ Proof.
 Qed.
 
 Definition add_suc_l_spec: Prop. 
-Proof. now unshelve refine (forall (m:{m: Natural| True}) (n:{n: Natural| True}), Suc (` (add m n))=(` (add (injectionCast Natural (fun m: Natural => True) (Suc (` (m))) _) n))). .
+Proof. smt_now unshelve refine (forall (m:{m: Natural| True}) (n:{n: Natural| True}), (Suc (` (add m n))=(` (add (injectionCast Natural (fun m: Natural => True) (Suc (` (m))) _) n)))). 
 Defined.
 Theorem add_suc_l: add_suc_l_spec.
 Proof.
@@ -70,8 +152,19 @@ Proof.
     { smt_app IHm. }
 Qed.
 
+Definition add_mono_r_spec: Prop. 
+Proof. smt_now unshelve refine (forall (m:{m: Natural| True}) (n:{n: Natural| True}), geqN (subsumptionCast Natural (fun VV: Natural => ((` (add_unrefined m n))=(VV))) (fun m: Natural => True) _ (add m n)) m /\ geN n (injectionCast Natural (fun n: Natural => True) (ZeroN) _)->geN (subsumptionCast Natural (fun VV: Natural => ((` (add_unrefined m n))=(VV))) (fun m: Natural => True) _ (add m n)) m). 
+Defined.
+Theorem add_mono_r: add_mono_r_spec.
+Proof.
+  intros m. intros n. destruct m as [m mp ].  destruct n as [n np ]. 
+  induction m as [| m IHm ]. 
+    { smt_now smt_trivial. }
+    { smt_app (add_suc_l (injectionCast Natural (fun m: Natural => True) (m) _) (injectionCast Natural (fun n: Natural => True) (n) _)). smt_app IHm. }
+Qed.
+
 Definition add_zero_r_spec: Prop. 
-Proof. now unshelve refine (forall (n:{n: Natural| True}), (` (add n (injectionCast Natural (fun n: Natural => True) (ZeroN) _)))=(` (n))). .
+Proof. smt_now unshelve refine (forall (n:{n: Natural| True}), ((` (add n (injectionCast Natural (fun n: Natural => True) (ZeroN) _)))=(` (n)))). 
 Defined.
 Theorem add_zero_r: add_zero_r_spec.
 Proof.
@@ -82,7 +175,7 @@ Proof.
 Qed.
 
 Definition mult_one_l_spec: Prop. 
-Proof. now unshelve refine (forall (n:{n: Natural| True}), (` (mult (injectionCast Natural (fun m: Natural => True) (one) _) n))=(` (n))). .
+Proof. smt_now unshelve refine (forall (n:{n: Natural| True}), ((` (mult (injectionCast Natural (fun m: Natural => True) (one) _) n))=(` (n)))). 
 Defined.
 Theorem mult_one_l: mult_one_l_spec.
 Proof.
@@ -92,7 +185,7 @@ Proof.
 Qed.
 
 Definition add_suc_r_spec: Prop. 
-Proof. now unshelve refine (forall (m:{m: Natural| True}) (n:{n: Natural| True}), Suc (` (add m n))=(` (add m (injectionCast Natural (fun n: Natural => True) (Suc (` (n))) _)))). .
+Proof. smt_now unshelve refine (forall (m:{m: Natural| True}) (n:{n: Natural| True}), (Suc (` (add m n))=(` (add m (injectionCast Natural (fun n: Natural => True) (Suc (` (n))) _))))). 
 Defined.
 Theorem add_suc_r: add_suc_r_spec.
 Proof.
@@ -103,7 +196,7 @@ Proof.
 Qed.
 
 Definition add_comm_spec: Prop. 
-Proof. now unshelve refine (forall (m:{m: Natural| True}) (n:{n: Natural| True}), (` (add m n))=(` (add n m))). .
+Proof. smt_now unshelve refine (forall (m:{m: Natural| True}) (n:{n: Natural| True}), ((` (add m n))=(` (add n m)))). 
 Defined.
 Theorem add_comm: add_comm_spec.
 Proof.
@@ -113,8 +206,29 @@ Proof.
     { smt_app IHm. smt_app (add_suc_r (injectionCast Natural (fun m: Natural => True) (n) _) (injectionCast Natural (fun n: Natural => True) (m) _)). }
 Qed.
 
+Definition add_mono_l_spec: Prop. 
+Proof. smt_now unshelve refine (forall (m:{m: Natural| True}) (n:{n: Natural| True}), geqN (subsumptionCast Natural (fun VV: Natural => ((` (add_unrefined m n))=(VV))) (fun m: Natural => True) _ (add m n)) n /\ geN m (injectionCast Natural (fun n: Natural => True) (ZeroN) _)->geN (subsumptionCast Natural (fun VV: Natural => ((` (add_unrefined m n))=(VV))) (fun m: Natural => True) _ (add m n)) n). 
+Defined.
+Theorem add_mono_l: add_mono_l_spec.
+Proof.
+  intros m. intros n. destruct m as [m mp ].  destruct n as [n np ]. 
+  
+    { smt_app (add_mono_r (injectionCast Natural (fun m: Natural => True) (n) _) (injectionCast Natural (fun n: Natural => True) (m) _)). smt_app (add_comm (injectionCast Natural (fun m: Natural => True) (n) _) (injectionCast Natural (fun n: Natural => True) (m) _)). }
+Qed.
+
+Definition add_subt_spec: Prop. 
+Proof. smt_now unshelve refine (forall (m:{m: Natural| True}) (n:{n: Natural| True}), ((` (subt (subsumptionCast Natural (fun VV: Natural => ((` (add_unrefined m n))=(VV))) (fun m: Natural => True) _ (add m n)) (subsumptionCast Natural (fun n: Natural => True) (fun n: Natural => geqN m n) _ (n))))=(` (m)))). 
+Defined.
+Theorem add_subt: add_subt_spec.
+Proof.
+  intros m. intros n. destruct m as [m mp ].  destruct n as [n np ]. 
+  induction m as [| m IHm ]. 
+    { destruct n as [ | lq_anf7205759403792798452 ]. smt_now smt_trivial. destruct n as [ | n ]. destruct () as [ ]. smt_app (add_suc_r (injectionCast Natural (fun m: Natural => True) (m) _) (injectionCast Natural (fun n: Natural => True) (n) _)). smt_app (add_subt (injectionCast Natural (fun m: Natural => True) (m) _) (injectionCast Natural (fun n: Natural => True) (n) _)). }
+    { destruct n as [ | lq_anf7205759403792798460 ]. smt_app (add_zero_r (injectionCast Natural (fun n: Natural => True) (m) _)). destruct n as [ | n ]. destruct () as [ ]. smt_app (add_suc_r (injectionCast Natural (fun m: Natural => True) (m) _) (injectionCast Natural (fun n: Natural => True) (n) _)). smt_app IHm. }
+Qed.
+
 Definition add_assoc_spec: Prop. 
-Proof. smt_now unshelve refine (forall (m:{m: Natural| True}) (n:{n: Natural| True}) (o:{o: Natural| True}), (` (add m (subsumptionCast Natural (fun VV: Natural => (` (add_unrefined m n))=VV) (fun n: Natural => True) _ (add n o))))=(` (add (subsumptionCast Natural (fun VV: Natural => (` (add_unrefined m n))=VV) (fun m: Natural => True) _ (add m n)) o))). .
+Proof. smt_now unshelve refine (forall (m:{m: Natural| True}) (n:{n: Natural| True}) (o:{o: Natural| True}), ((` (add m (subsumptionCast Natural (fun VV: Natural => ((` (add_unrefined m n))=(VV))) (fun n: Natural => True) _ (add n o))))=(` (add (subsumptionCast Natural (fun VV: Natural => ((` (add_unrefined m n))=(VV))) (fun m: Natural => True) _ (add m n)) o)))). 
 Defined.
 Theorem add_assoc: add_assoc_spec.
 Proof.
@@ -125,29 +239,29 @@ Proof.
 Qed.
 
 Definition mult_suc_r_spec: Prop. 
-Proof. now unshelve refine (forall (n:{n: Natural| True}) (m:{m: Natural| True}), (` (mult n (injectionCast Natural (fun n: Natural => True) (Suc (` (m))) _)))=(` (add n (subsumptionCast Natural (fun VV: Natural => (` (mult_unrefined m n))=VV) (fun n: Natural => True) _ (mult n m))))). .
+Proof. smt_now unshelve refine (forall (n:{n: Natural| True}) (m:{m: Natural| True}), ((` (mult n (injectionCast Natural (fun n: Natural => True) (Suc (` (m))) _)))=(` (add n (subsumptionCast Natural (fun VV: Natural => ((` (mult_unrefined m n))=(VV))) (fun n: Natural => True) _ (mult n m)))))). 
 Defined.
 Theorem mult_suc_r: mult_suc_r_spec.
 Proof.
   intros n. intros m. destruct n as [n np ].  destruct m as [m mp ]. 
   induction n as [| n IHn ]. 
     { smt_now smt_trivial. }
-    { smt_app IHn. smt_app (add_assoc (injectionCast Natural (fun m: Natural => True) (m) _) (injectionCast Natural (fun n: Natural => True) (n) _) (subsumptionCast Natural (fun VV: Natural => (` (mult_unrefined (injectionCast Natural (fun m: Natural => True) (m) _) (injectionCast Natural (fun n: Natural => True) (n) _)))=VV) (fun o: Natural => True) _ (mult (injectionCast Natural (fun m: Natural => True) (n) _) (injectionCast Natural (fun n: Natural => True) (m) _)))). smt_app (add_comm (injectionCast Natural (fun m: Natural => True) (m) _) (injectionCast Natural (fun n: Natural => True) (n) _)). smt_app (add_assoc (injectionCast Natural (fun m: Natural => True) (n) _) (injectionCast Natural (fun n: Natural => True) (m) _) (subsumptionCast Natural (fun VV: Natural => (` (mult_unrefined (injectionCast Natural (fun m: Natural => True) (m) _) (injectionCast Natural (fun n: Natural => True) (n) _)))=VV) (fun o: Natural => True) _ (mult (injectionCast Natural (fun m: Natural => True) (n) _) (injectionCast Natural (fun n: Natural => True) (m) _)))). }
+    { smt_app IHn. smt_app (add_assoc (injectionCast Natural (fun m: Natural => True) (m) _) (injectionCast Natural (fun n: Natural => True) (n) _) (subsumptionCast Natural (fun VV: Natural => ((` (mult_unrefined (injectionCast Natural (fun m: Natural => True) (m) _) (injectionCast Natural (fun n: Natural => True) (n) _)))=(VV))) (fun o: Natural => True) _ (mult (injectionCast Natural (fun m: Natural => True) (n) _) (injectionCast Natural (fun n: Natural => True) (m) _)))). smt_app (add_comm (injectionCast Natural (fun m: Natural => True) (m) _) (injectionCast Natural (fun n: Natural => True) (n) _)). smt_app (add_assoc (injectionCast Natural (fun m: Natural => True) (n) _) (injectionCast Natural (fun n: Natural => True) (m) _) (subsumptionCast Natural (fun VV: Natural => ((` (mult_unrefined (injectionCast Natural (fun m: Natural => True) (m) _) (injectionCast Natural (fun n: Natural => True) (n) _)))=(VV))) (fun o: Natural => True) _ (mult (injectionCast Natural (fun m: Natural => True) (n) _) (injectionCast Natural (fun n: Natural => True) (m) _)))). }
 Qed.
 
 Definition add_dist_rmult_spec: Prop. 
-Proof. now unshelve refine (forall (m:{m: Natural| True}) (n:{n: Natural| True}) (o:{o: Natural| True}), (` (mult (subsumptionCast Natural (fun VV: Natural => (` (add_unrefined m n))=VV) (fun m: Natural => True) _ (add m n)) o))=(` (add (subsumptionCast Natural (fun VV: Natural => (` (mult_unrefined m n))=VV) (fun m: Natural => True) _ (mult m o)) (subsumptionCast Natural (fun VV: Natural => (` (mult_unrefined m n))=VV) (fun n: Natural => True) _ (mult n o))))). .
+Proof. smt_now unshelve refine (forall (m:{m: Natural| True}) (n:{n: Natural| True}) (o:{o: Natural| True}), ((` (mult (subsumptionCast Natural (fun VV: Natural => ((` (add_unrefined m n))=(VV))) (fun m: Natural => True) _ (add m n)) o))=(` (add (subsumptionCast Natural (fun VV: Natural => ((` (mult_unrefined m n))=(VV))) (fun m: Natural => True) _ (mult m o)) (subsumptionCast Natural (fun VV: Natural => ((` (mult_unrefined m n))=(VV))) (fun n: Natural => True) _ (mult n o)))))). 
 Defined.
 Theorem add_dist_rmult: add_dist_rmult_spec.
 Proof.
   intros m. intros n. intros o. destruct m as [m mp ].  destruct n as [n np ].  destruct o as [o op ]. 
   induction m as [| m IHm ]. 
     { smt_now smt_trivial. }
-    { smt_app IHm. smt_app (add_assoc (injectionCast Natural (fun m: Natural => True) (o) _) (subsumptionCast Natural (fun VV: Natural => (` (mult_unrefined (injectionCast Natural (fun m: Natural => True) (m) _) (injectionCast Natural (fun n: Natural => True) (n) _)))=VV) (fun n: Natural => True) _ (mult (injectionCast Natural (fun m: Natural => True) (m) _) (injectionCast Natural (fun n: Natural => True) (o) _))) (subsumptionCast Natural (fun VV: Natural => (` (mult_unrefined (injectionCast Natural (fun m: Natural => True) (m) _) (injectionCast Natural (fun n: Natural => True) (n) _)))=VV) (fun o: Natural => True) _ (mult (injectionCast Natural (fun m: Natural => True) (n) _) (injectionCast Natural (fun n: Natural => True) (o) _)))). }
+    { smt_app IHm. smt_app (add_assoc (injectionCast Natural (fun m: Natural => True) (o) _) (subsumptionCast Natural (fun VV: Natural => ((` (mult_unrefined (injectionCast Natural (fun m: Natural => True) (m) _) (injectionCast Natural (fun n: Natural => True) (n) _)))=(VV))) (fun n: Natural => True) _ (mult (injectionCast Natural (fun m: Natural => True) (m) _) (injectionCast Natural (fun n: Natural => True) (o) _))) (subsumptionCast Natural (fun VV: Natural => ((` (mult_unrefined (injectionCast Natural (fun m: Natural => True) (m) _) (injectionCast Natural (fun n: Natural => True) (n) _)))=(VV))) (fun o: Natural => True) _ (mult (injectionCast Natural (fun m: Natural => True) (n) _) (injectionCast Natural (fun n: Natural => True) (o) _)))). }
 Qed.
 
 Definition mult_assoc_spec: Prop. 
-Proof. now unshelve refine (forall (m:{m: Natural| True}) (n:{n: Natural| True}) (o:{o: Natural| True}), (` (mult (subsumptionCast Natural (fun VV: Natural => (` (mult_unrefined m n))=VV) (fun m: Natural => True) _ (mult m n)) o))=(` (mult m (subsumptionCast Natural (fun VV: Natural => (` (mult_unrefined m n))=VV) (fun n: Natural => True) _ (mult n o))))). .
+Proof. smt_now unshelve refine (forall (m:{m: Natural| True}) (n:{n: Natural| True}) (o:{o: Natural| True}), ((` (mult (subsumptionCast Natural (fun VV: Natural => ((` (mult_unrefined m n))=(VV))) (fun m: Natural => True) _ (mult m n)) o))=(` (mult m (subsumptionCast Natural (fun VV: Natural => ((` (mult_unrefined m n))=(VV))) (fun n: Natural => True) _ (mult n o)))))). 
 Defined.
 Theorem mult_assoc: mult_assoc_spec.
 Proof.
@@ -155,14 +269,14 @@ Proof.
   induction m as [| m IHm ]. 
     { smt_now smt_trivial. }
     { 
-  assertFresh ((` (mult (subsumptionCast Natural (fun VV: Natural => (` (mult_unrefined (injectionCast Natural (fun m: Natural => True) (m) _) (injectionCast Natural (fun n: Natural => True) (n) _)))=VV) (fun m: Natural => True) _ (mult (injectionCast Natural (fun m: Natural => True) (Suc m) _) (injectionCast Natural (fun n: Natural => True) (n) _))) (injectionCast Natural (fun n: Natural => True) (o) _)))=(` (mult (subsumptionCast Natural (fun VV: Natural => (` (add_unrefined (injectionCast Natural (fun m: Natural => True) (m) _) (injectionCast Natural (fun n: Natural => True) (n) _)))=VV) (fun m: Natural => True) _ (add (injectionCast Natural (fun m: Natural => True) (n) _) (subsumptionCast Natural (fun VV: Natural => (` (mult_unrefined (injectionCast Natural (fun m: Natural => True) (m) _) (injectionCast Natural (fun n: Natural => True) (n) _)))=VV) (fun n: Natural => True) _ (mult (injectionCast Natural (fun m: Natural => True) (m) _) (injectionCast Natural (fun n: Natural => True) (n) _))))) (injectionCast Natural (fun n: Natural => True) (o) _)))) as lem using smt_trivial. . 
-  assertFresh ((` (mult (subsumptionCast Natural (fun VV: Natural => (` (add_unrefined (injectionCast Natural (fun m: Natural => True) (m) _) (injectionCast Natural (fun n: Natural => True) (n) _)))=VV) (fun m: Natural => True) _ (add (injectionCast Natural (fun m: Natural => True) (n) _) (subsumptionCast Natural (fun VV: Natural => (` (mult_unrefined (injectionCast Natural (fun m: Natural => True) (m) _) (injectionCast Natural (fun n: Natural => True) (n) _)))=VV) (fun n: Natural => True) _ (mult (injectionCast Natural (fun m: Natural => True) (m) _) (injectionCast Natural (fun n: Natural => True) (n) _))))) (injectionCast Natural (fun n: Natural => True) (o) _)))=(` (add (subsumptionCast Natural (fun VV: Natural => (` (mult_unrefined (injectionCast Natural (fun m: Natural => True) (m) _) (injectionCast Natural (fun n: Natural => True) (n) _)))=VV) (fun m: Natural => True) _ (mult (injectionCast Natural (fun m: Natural => True) (n) _) (injectionCast Natural (fun n: Natural => True) (o) _))) (subsumptionCast Natural (fun VV: Natural => (` (mult_unrefined (injectionCast Natural (fun m: Natural => True) (m) _) (injectionCast Natural (fun n: Natural => True) (n) _)))=VV) (fun n: Natural => True) _ (mult (subsumptionCast Natural (fun VV: Natural => (` (mult_unrefined (injectionCast Natural (fun m: Natural => True) (m) _) (injectionCast Natural (fun n: Natural => True) (n) _)))=VV) (fun m: Natural => True) _ (mult (injectionCast Natural (fun m: Natural => True) (m) _) (injectionCast Natural (fun n: Natural => True) (n) _))) (injectionCast Natural (fun n: Natural => True) (o) _)))))) as lem using (smt_app (add_dist_rmult (injectionCast Natural (fun m: Natural => True) (n) _) (subsumptionCast Natural (fun VV: Natural => (` (mult_unrefined (injectionCast Natural (fun m: Natural => True) (m) _) (injectionCast Natural (fun n: Natural => True) (n) _)))=VV) (fun n: Natural => True) _ (mult (injectionCast Natural (fun m: Natural => True) (m) _) (injectionCast Natural (fun n: Natural => True) (n) _))) (injectionCast Natural (fun o: Natural => True) (o) _)). ). 
-  assertFresh ((` (add (subsumptionCast Natural (fun VV: Natural => (` (mult_unrefined (injectionCast Natural (fun m: Natural => True) (m) _) (injectionCast Natural (fun n: Natural => True) (n) _)))=VV) (fun m: Natural => True) _ (mult (injectionCast Natural (fun m: Natural => True) (n) _) (injectionCast Natural (fun n: Natural => True) (o) _))) (subsumptionCast Natural (fun VV: Natural => (` (mult_unrefined (injectionCast Natural (fun m: Natural => True) (m) _) (injectionCast Natural (fun n: Natural => True) (n) _)))=VV) (fun n: Natural => True) _ (mult (subsumptionCast Natural (fun VV: Natural => (` (mult_unrefined (injectionCast Natural (fun m: Natural => True) (m) _) (injectionCast Natural (fun n: Natural => True) (n) _)))=VV) (fun m: Natural => True) _ (mult (injectionCast Natural (fun m: Natural => True) (m) _) (injectionCast Natural (fun n: Natural => True) (n) _))) (injectionCast Natural (fun n: Natural => True) (o) _)))))=(` (add (subsumptionCast Natural (fun VV: Natural => (` (mult_unrefined (injectionCast Natural (fun m: Natural => True) (m) _) (injectionCast Natural (fun n: Natural => True) (n) _)))=VV) (fun m: Natural => True) _ (mult (injectionCast Natural (fun m: Natural => True) (n) _) (injectionCast Natural (fun n: Natural => True) (o) _))) (subsumptionCast Natural (fun VV: Natural => (` (mult_unrefined (injectionCast Natural (fun m: Natural => True) (m) _) (injectionCast Natural (fun n: Natural => True) (n) _)))=VV) (fun n: Natural => True) _ (mult (injectionCast Natural (fun m: Natural => True) (m) _) (subsumptionCast Natural (fun VV: Natural => (` (mult_unrefined (injectionCast Natural (fun m: Natural => True) (m) _) (injectionCast Natural (fun n: Natural => True) (n) _)))=VV) (fun n: Natural => True) _ (mult (injectionCast Natural (fun m: Natural => True) (n) _) (injectionCast Natural (fun n: Natural => True) (o) _)))))))) as lem using (smt_app IHm. ). smt_now 
-  assertFresh ((` (add (subsumptionCast Natural (fun VV: Natural => (` (mult_unrefined (injectionCast Natural (fun m: Natural => True) (m) _) (injectionCast Natural (fun n: Natural => True) (n) _)))=VV) (fun m: Natural => True) _ (mult (injectionCast Natural (fun m: Natural => True) (n) _) (injectionCast Natural (fun n: Natural => True) (o) _))) (subsumptionCast Natural (fun VV: Natural => (` (mult_unrefined (injectionCast Natural (fun m: Natural => True) (m) _) (injectionCast Natural (fun n: Natural => True) (n) _)))=VV) (fun n: Natural => True) _ (mult (injectionCast Natural (fun m: Natural => True) (m) _) (subsumptionCast Natural (fun VV: Natural => (` (mult_unrefined (injectionCast Natural (fun m: Natural => True) (m) _) (injectionCast Natural (fun n: Natural => True) (n) _)))=VV) (fun n: Natural => True) _ (mult (injectionCast Natural (fun m: Natural => True) (n) _) (injectionCast Natural (fun n: Natural => True) (o) _)))))))=(` (mult (injectionCast Natural (fun m: Natural => True) (Suc m) _) (subsumptionCast Natural (fun VV: Natural => (` (mult_unrefined (injectionCast Natural (fun m: Natural => True) (m) _) (injectionCast Natural (fun n: Natural => True) (n) _)))=VV) (fun n: Natural => True) _ (mult (injectionCast Natural (fun m: Natural => True) (n) _) (injectionCast Natural (fun n: Natural => True) (o) _)))))) as lem using smt_trivial. . }
+  assertFresh ((` (mult (subsumptionCast Natural (fun VV: Natural => ((` (mult_unrefined (injectionCast Natural (fun m: Natural => True) (m) _) (injectionCast Natural (fun n: Natural => True) (n) _)))=(VV))) (fun m: Natural => True) _ (mult (injectionCast Natural (fun m: Natural => True) (Suc m) _) (injectionCast Natural (fun n: Natural => True) (n) _))) (injectionCast Natural (fun n: Natural => True) (o) _)))=(` (mult (subsumptionCast Natural (fun VV: Natural => ((` (add_unrefined (injectionCast Natural (fun m: Natural => True) (m) _) (injectionCast Natural (fun n: Natural => True) (n) _)))=(VV))) (fun m: Natural => True) _ (add (injectionCast Natural (fun m: Natural => True) (n) _) (subsumptionCast Natural (fun VV: Natural => ((` (mult_unrefined (injectionCast Natural (fun m: Natural => True) (m) _) (injectionCast Natural (fun n: Natural => True) (n) _)))=(VV))) (fun n: Natural => True) _ (mult (injectionCast Natural (fun m: Natural => True) (m) _) (injectionCast Natural (fun n: Natural => True) (n) _))))) (injectionCast Natural (fun n: Natural => True) (o) _)))) as lem using smt_trivial. . 
+  assertFresh ((` (mult (subsumptionCast Natural (fun VV: Natural => ((` (add_unrefined (injectionCast Natural (fun m: Natural => True) (m) _) (injectionCast Natural (fun n: Natural => True) (n) _)))=(VV))) (fun m: Natural => True) _ (add (injectionCast Natural (fun m: Natural => True) (n) _) (subsumptionCast Natural (fun VV: Natural => ((` (mult_unrefined (injectionCast Natural (fun m: Natural => True) (m) _) (injectionCast Natural (fun n: Natural => True) (n) _)))=(VV))) (fun n: Natural => True) _ (mult (injectionCast Natural (fun m: Natural => True) (m) _) (injectionCast Natural (fun n: Natural => True) (n) _))))) (injectionCast Natural (fun n: Natural => True) (o) _)))=(` (add (subsumptionCast Natural (fun VV: Natural => ((` (mult_unrefined (injectionCast Natural (fun m: Natural => True) (m) _) (injectionCast Natural (fun n: Natural => True) (n) _)))=(VV))) (fun m: Natural => True) _ (mult (injectionCast Natural (fun m: Natural => True) (n) _) (injectionCast Natural (fun n: Natural => True) (o) _))) (subsumptionCast Natural (fun VV: Natural => ((` (mult_unrefined (injectionCast Natural (fun m: Natural => True) (m) _) (injectionCast Natural (fun n: Natural => True) (n) _)))=(VV))) (fun n: Natural => True) _ (mult (subsumptionCast Natural (fun VV: Natural => ((` (mult_unrefined (injectionCast Natural (fun m: Natural => True) (m) _) (injectionCast Natural (fun n: Natural => True) (n) _)))=(VV))) (fun m: Natural => True) _ (mult (injectionCast Natural (fun m: Natural => True) (m) _) (injectionCast Natural (fun n: Natural => True) (n) _))) (injectionCast Natural (fun n: Natural => True) (o) _)))))) as lem using (smt_app (add_dist_rmult (injectionCast Natural (fun m: Natural => True) (n) _) (subsumptionCast Natural (fun VV: Natural => ((` (mult_unrefined (injectionCast Natural (fun m: Natural => True) (m) _) (injectionCast Natural (fun n: Natural => True) (n) _)))=(VV))) (fun n: Natural => True) _ (mult (injectionCast Natural (fun m: Natural => True) (m) _) (injectionCast Natural (fun n: Natural => True) (n) _))) (injectionCast Natural (fun o: Natural => True) (o) _)). ). 
+  assertFresh ((` (add (subsumptionCast Natural (fun VV: Natural => ((` (mult_unrefined (injectionCast Natural (fun m: Natural => True) (m) _) (injectionCast Natural (fun n: Natural => True) (n) _)))=(VV))) (fun m: Natural => True) _ (mult (injectionCast Natural (fun m: Natural => True) (n) _) (injectionCast Natural (fun n: Natural => True) (o) _))) (subsumptionCast Natural (fun VV: Natural => ((` (mult_unrefined (injectionCast Natural (fun m: Natural => True) (m) _) (injectionCast Natural (fun n: Natural => True) (n) _)))=(VV))) (fun n: Natural => True) _ (mult (subsumptionCast Natural (fun VV: Natural => ((` (mult_unrefined (injectionCast Natural (fun m: Natural => True) (m) _) (injectionCast Natural (fun n: Natural => True) (n) _)))=(VV))) (fun m: Natural => True) _ (mult (injectionCast Natural (fun m: Natural => True) (m) _) (injectionCast Natural (fun n: Natural => True) (n) _))) (injectionCast Natural (fun n: Natural => True) (o) _)))))=(` (add (subsumptionCast Natural (fun VV: Natural => ((` (mult_unrefined (injectionCast Natural (fun m: Natural => True) (m) _) (injectionCast Natural (fun n: Natural => True) (n) _)))=(VV))) (fun m: Natural => True) _ (mult (injectionCast Natural (fun m: Natural => True) (n) _) (injectionCast Natural (fun n: Natural => True) (o) _))) (subsumptionCast Natural (fun VV: Natural => ((` (mult_unrefined (injectionCast Natural (fun m: Natural => True) (m) _) (injectionCast Natural (fun n: Natural => True) (n) _)))=(VV))) (fun n: Natural => True) _ (mult (injectionCast Natural (fun m: Natural => True) (m) _) (subsumptionCast Natural (fun VV: Natural => ((` (mult_unrefined (injectionCast Natural (fun m: Natural => True) (m) _) (injectionCast Natural (fun n: Natural => True) (n) _)))=(VV))) (fun n: Natural => True) _ (mult (injectionCast Natural (fun m: Natural => True) (n) _) (injectionCast Natural (fun n: Natural => True) (o) _)))))))) as lem using (smt_app IHm. ). smt_now 
+  assertFresh ((` (add (subsumptionCast Natural (fun VV: Natural => ((` (mult_unrefined (injectionCast Natural (fun m: Natural => True) (m) _) (injectionCast Natural (fun n: Natural => True) (n) _)))=(VV))) (fun m: Natural => True) _ (mult (injectionCast Natural (fun m: Natural => True) (n) _) (injectionCast Natural (fun n: Natural => True) (o) _))) (subsumptionCast Natural (fun VV: Natural => ((` (mult_unrefined (injectionCast Natural (fun m: Natural => True) (m) _) (injectionCast Natural (fun n: Natural => True) (n) _)))=(VV))) (fun n: Natural => True) _ (mult (injectionCast Natural (fun m: Natural => True) (m) _) (subsumptionCast Natural (fun VV: Natural => ((` (mult_unrefined (injectionCast Natural (fun m: Natural => True) (m) _) (injectionCast Natural (fun n: Natural => True) (n) _)))=(VV))) (fun n: Natural => True) _ (mult (injectionCast Natural (fun m: Natural => True) (n) _) (injectionCast Natural (fun n: Natural => True) (o) _)))))))=(` (mult (injectionCast Natural (fun m: Natural => True) (Suc m) _) (subsumptionCast Natural (fun VV: Natural => ((` (mult_unrefined (injectionCast Natural (fun m: Natural => True) (m) _) (injectionCast Natural (fun n: Natural => True) (n) _)))=(VV))) (fun n: Natural => True) _ (mult (injectionCast Natural (fun m: Natural => True) (n) _) (injectionCast Natural (fun n: Natural => True) (o) _)))))) as lem using smt_trivial. . }
 Qed.
 
 Definition mult_zero_l_spec: Prop. 
-Proof. now unshelve refine (forall (n:{n: Natural| True}), (` (mult (injectionCast Natural (fun m: Natural => True) (ZeroN) _) n))=ZeroN). .
+Proof. smt_now unshelve refine (forall (n:{n: Natural| True}), ((` (mult (injectionCast Natural (fun m: Natural => True) (ZeroN) _) n))=(ZeroN))). 
 Defined.
 Theorem mult_zero_l: mult_zero_l_spec.
 Proof.
@@ -173,7 +287,7 @@ Proof.
 Qed.
 
 Definition mult_suc_l_spec: Prop. 
-Proof. now unshelve refine (forall (m:{m: Natural| True}) (n:{n: Natural| True}), (` (mult (injectionCast Natural (fun m: Natural => True) (Suc (` (m))) _) n))=(` (add n (subsumptionCast Natural (fun VV: Natural => (` (mult_unrefined m n))=VV) (fun n: Natural => True) _ (mult m n))))). .
+Proof. smt_now unshelve refine (forall (m:{m: Natural| True}) (n:{n: Natural| True}), ((` (mult (injectionCast Natural (fun m: Natural => True) (Suc (` (m))) _) n))=(` (add n (subsumptionCast Natural (fun VV: Natural => ((` (mult_unrefined m n))=(VV))) (fun n: Natural => True) _ (mult m n)))))). 
 Defined.
 Theorem mult_suc_l: mult_suc_l_spec.
 Proof.
@@ -183,7 +297,7 @@ Proof.
 Qed.
 
 Definition mult_zero_r_spec: Prop. 
-Proof. now unshelve refine (forall (n:{n: Natural| True}), (` (mult n (injectionCast Natural (fun n: Natural => True) (ZeroN) _)))=ZeroN). .
+Proof. smt_now unshelve refine (forall (n:{n: Natural| True}), ((` (mult n (injectionCast Natural (fun n: Natural => True) (ZeroN) _)))=(ZeroN))). 
 Defined.
 Theorem mult_zero_r: mult_zero_r_spec.
 Proof.
@@ -194,18 +308,18 @@ Proof.
 Qed.
 
 Definition add_dist_lmult_spec: Prop. 
-Proof. now unshelve refine (forall (m:{m: Natural| True}) (n:{n: Natural| True}) (o:{o: Natural| True}), (` (mult m (subsumptionCast Natural (fun VV: Natural => (` (add_unrefined m n))=VV) (fun n: Natural => True) _ (add n o))))=(` (add (subsumptionCast Natural (fun VV: Natural => (` (mult_unrefined m n))=VV) (fun m: Natural => True) _ (mult m n)) (subsumptionCast Natural (fun VV: Natural => (` (mult_unrefined m n))=VV) (fun n: Natural => True) _ (mult m o))))). .
+Proof. smt_now unshelve refine (forall (m:{m: Natural| True}) (n:{n: Natural| True}) (o:{o: Natural| True}), ((` (mult m (subsumptionCast Natural (fun VV: Natural => ((` (add_unrefined m n))=(VV))) (fun n: Natural => True) _ (add n o))))=(` (add (subsumptionCast Natural (fun VV: Natural => ((` (mult_unrefined m n))=(VV))) (fun m: Natural => True) _ (mult m n)) (subsumptionCast Natural (fun VV: Natural => ((` (mult_unrefined m n))=(VV))) (fun n: Natural => True) _ (mult m o)))))). 
 Defined.
 Theorem add_dist_lmult: add_dist_lmult_spec.
 Proof.
   intros m. intros n. intros o. destruct m as [m mp ].  destruct n as [n np ].  destruct o as [o op ]. 
   induction n as [| n IHn ]. 
     { smt_app (mult_zero_r (injectionCast Natural (fun n: Natural => True) (m) _)). }
-    { smt_app (mult_suc_r (injectionCast Natural (fun n: Natural => True) (m) _) (subsumptionCast Natural (fun VV: Natural => (` (add_unrefined (injectionCast Natural (fun m: Natural => True) (m) _) (injectionCast Natural (fun n: Natural => True) (n) _)))=VV) (fun m: Natural => True) _ (add (injectionCast Natural (fun m: Natural => True) (n) _) (injectionCast Natural (fun n: Natural => True) (o) _)))). smt_app IHn. smt_app (add_assoc (injectionCast Natural (fun m: Natural => True) (m) _) (subsumptionCast Natural (fun VV: Natural => (` (mult_unrefined (injectionCast Natural (fun m: Natural => True) (m) _) (injectionCast Natural (fun n: Natural => True) (n) _)))=VV) (fun n: Natural => True) _ (mult (injectionCast Natural (fun m: Natural => True) (m) _) (injectionCast Natural (fun n: Natural => True) (n) _))) (subsumptionCast Natural (fun VV: Natural => (` (mult_unrefined (injectionCast Natural (fun m: Natural => True) (m) _) (injectionCast Natural (fun n: Natural => True) (n) _)))=VV) (fun o: Natural => True) _ (mult (injectionCast Natural (fun m: Natural => True) (m) _) (injectionCast Natural (fun n: Natural => True) (o) _)))). smt_app (mult_suc_r (injectionCast Natural (fun n: Natural => True) (m) _) (injectionCast Natural (fun m: Natural => True) (n) _)). }
+    { smt_app (mult_suc_r (injectionCast Natural (fun n: Natural => True) (m) _) (subsumptionCast Natural (fun VV: Natural => ((` (add_unrefined (injectionCast Natural (fun m: Natural => True) (m) _) (injectionCast Natural (fun n: Natural => True) (n) _)))=(VV))) (fun m: Natural => True) _ (add (injectionCast Natural (fun m: Natural => True) (n) _) (injectionCast Natural (fun n: Natural => True) (o) _)))). smt_app IHn. smt_app (add_assoc (injectionCast Natural (fun m: Natural => True) (m) _) (subsumptionCast Natural (fun VV: Natural => ((` (mult_unrefined (injectionCast Natural (fun m: Natural => True) (m) _) (injectionCast Natural (fun n: Natural => True) (n) _)))=(VV))) (fun n: Natural => True) _ (mult (injectionCast Natural (fun m: Natural => True) (m) _) (injectionCast Natural (fun n: Natural => True) (n) _))) (subsumptionCast Natural (fun VV: Natural => ((` (mult_unrefined (injectionCast Natural (fun m: Natural => True) (m) _) (injectionCast Natural (fun n: Natural => True) (n) _)))=(VV))) (fun o: Natural => True) _ (mult (injectionCast Natural (fun m: Natural => True) (m) _) (injectionCast Natural (fun n: Natural => True) (o) _)))). smt_app (mult_suc_r (injectionCast Natural (fun n: Natural => True) (m) _) (injectionCast Natural (fun m: Natural => True) (n) _)). }
 Qed.
 
 Definition mult_one_r_spec: Prop. 
-Proof. now unshelve refine (forall (n:{n: Natural| True}), (` (mult n (injectionCast Natural (fun n: Natural => True) (one) _)))=(` (n))). .
+Proof. smt_now unshelve refine (forall (n:{n: Natural| True}), ((` (mult n (injectionCast Natural (fun n: Natural => True) (one) _)))=(` (n)))). 
 Defined.
 Theorem mult_one_r: mult_one_r_spec.
 Proof.
@@ -213,4 +327,311 @@ Proof.
   induction n as [| n IHn ]. 
     { smt_now smt_trivial. }
     { smt_app IHn. }
+Qed.
+
+Definition ge_measure_spec: Prop. 
+Proof. smt_now unshelve refine (forall (m:{m: Natural| True}) (n:{n: Natural| True}), ((` (geN m n))=((` (toInt m))>(` (toInt n))))). 
+Defined.
+Theorem ge_measure: ge_measure_spec.
+Proof.
+  intros m. intros n. destruct m as [m mp ].  destruct n as [n np ]. 
+  induction m as [| ds_d1e1 IHds_d1e1 ]. 
+    { smt_now smt_trivial. }
+    { destruct n as [ | n ]. smt_now smt_trivial. smt_app IHds_d1e1. }
+Qed.
+
+Definition ge_geq_suc_spec: Prop. 
+Proof. smt_now unshelve refine (forall (m:{m: Natural| True}) (n:{n: Natural| True}), ((` (geN m n))=(` (geqN m (injectionCast Natural (fun n: Natural => True) (Suc (` (n))) _))))). 
+Defined.
+Theorem ge_geq_suc: ge_geq_suc_spec.
+Proof.
+  intros m. intros n. destruct m as [m mp ].  destruct n as [n np ]. 
+  induction m as [| m IHm ]. 
+    { smt_now smt_trivial. }
+    { destruct n as [ | n ]. smt_now smt_trivial. smt_app IHm. }
+Qed.
+
+Definition ge_zero_spec: Prop. 
+Proof. smt_now unshelve refine (forall (n:{n: Natural| True}), geqN n (injectionCast Natural (fun n: Natural => True) (ZeroN) _) /\ ((` (n))<>(ZeroN))->geN n (injectionCast Natural (fun n: Natural => True) (ZeroN) _)). 
+Defined.
+Theorem ge_zero: ge_zero_spec.
+Proof.
+  intros n. destruct n as [n np ]. 
+  induction n as [| n IHn ]. 
+    { smt_now smt_trivial. }
+    { smt_app IHn. smt_app (ge_geq_suc (injectionCast Natural (fun m: Natural => True) (n) _) (injectionCast Natural (fun n: Natural => True) (ZeroN) _)). }
+Qed.
+
+Definition eq_suc_ge_spec: Prop. 
+Proof. smt_now unshelve refine (forall (m:{m: Natural| True}) (n:{n: Natural| True}), eqN m n->geN (injectionCast Natural (fun m: Natural => True) (Suc (` (m))) _) n). 
+Defined.
+Theorem eq_suc_ge: eq_suc_ge_spec.
+Proof.
+  intros m. intros n. destruct m as [m mp ].  destruct n as [n np ]. 
+  induction m as [| m IHm ]. 
+    { destruct n as [ | n ]. smt_now smt_trivial. smt_now smt_trivial. }
+    { destruct n as [ | n ]. smt_now smt_trivial. smt_app IHm. }
+Qed.
+
+Definition eq_equal_spec: Prop. 
+Proof. smt_now unshelve refine (forall (m:{m: Natural| True}) (n:{n: Natural| True}), ((` (eqN m n))=((` (m))=(` (n))))). 
+Defined.
+Theorem eq_equal: eq_equal_spec.
+Proof.
+  intros m. intros n. destruct m as [m mp ].  destruct n as [n np ]. 
+  induction m as [| m IHm ]. 
+    { destruct n as [ | lq_anf7205759403792798546 ]. smt_now smt_trivial. smt_now smt_trivial. }
+    { destruct n as [ | n ]. smt_now smt_trivial. smt_app IHm. }
+Qed.
+
+Definition eq_sym_spec: Prop. 
+Proof. smt_now unshelve refine (forall (m:{m: Natural| True}) (n:{n: Natural| True}), ((` (eqN m n))=(` (eqN n m)))). 
+Defined.
+Theorem eq_sym: eq_sym_spec.
+Proof.
+  intros m. intros n. destruct m as [m mp ].  destruct n as [n np ]. 
+  
+    { smt_app (eq_equal (injectionCast Natural (fun m: Natural => True) (m) _) (injectionCast Natural (fun n: Natural => True) (n) _)). smt_app (eq_equal (injectionCast Natural (fun m: Natural => True) (n) _) (injectionCast Natural (fun n: Natural => True) (m) _)). }
+Qed.
+
+Definition eq_geq_spec: Prop. 
+Proof. smt_now unshelve refine (forall (m:{m: Natural| True}) (n:{n: Natural| True}), eqN m n->geqN m n). 
+Defined.
+Theorem eq_geq: eq_geq_spec.
+Proof.
+  intros m. intros n. destruct m as [m mp ].  destruct n as [n np ]. 
+  induction m as [| m IHm ]. 
+    { destruct n as [ | lq_anf7205759403792798561 ]. smt_now smt_trivial. destruct m as [ | lq_anf7205759403792798560 ]. destruct n as [ | ds_d1di ]. destruct () as [ ]. smt_now smt_trivial. destruct () as [ ]. }
+    { destruct n as [ | n ]. destruct n as [ | lq_anf7205759403792798573 ]. smt_now smt_trivial. destruct m as [ | lq_anf7205759403792798572 ]. destruct n as [ | ds_d1di ]. destruct () as [ ]. smt_now smt_trivial. destruct () as [ ]. smt_app IHm. }
+Qed.
+
+Definition geq_refl_spec: Prop. 
+Proof. smt_now unshelve refine (forall (n:{n: Natural| True}), geqN n n). 
+Defined.
+Theorem geq_refl: geq_refl_spec.
+Proof.
+  intros n. destruct n as [n np ]. 
+  induction n as [| n IHn ]. 
+    { smt_now smt_trivial. }
+    { smt_app IHn. }
+Qed.
+
+Definition geq_trans_spec: Prop. 
+Proof. smt_now unshelve refine (forall (m:{m: Natural| True}) (n:{n: Natural| True}) (o:{o: Natural| True}), geqN m n /\ geqN n o->geqN m o). 
+Defined.
+Theorem geq_trans: geq_trans_spec.
+Proof.
+  intros m. intros n. intros o. destruct m as [m mp ].  destruct n as [n np ].  destruct o as [o op ]. 
+  induction m as [| m IHm ]. 
+    { smt_now smt_trivial. }
+    { destruct n as [ | lq_anf7205759403792798586 ]. smt_now smt_trivial. destruct m as [ | m ]. smt_now smt_trivial. destruct n as [ | n ]. destruct () as [ ]. destruct o as [ | o ]. destruct () as [ ]. smt_app IHm. }
+Qed.
+
+Definition le_geq_spec: Prop. 
+Proof. smt_now unshelve refine (forall (m:{m: Natural| True}) (n:{n: Natural| True}), ((` (geqN m n))=(not(leN m n)))). 
+Defined.
+Theorem le_geq: le_geq_spec.
+Proof.
+  intros m. intros n. destruct m as [m mp ].  destruct n as [n np ]. 
+  induction m as [| m IHm ]. 
+    { smt_now smt_trivial. }
+    { destruct m as [ | m ]. destruct n as [ | n ]. destruct () as [ ]. smt_now smt_trivial. destruct n as [ | n ]. destruct () as [ ]. smt_app IHm. }
+Qed.
+
+Definition ge_geq_spec: Prop. 
+Proof. smt_now unshelve refine (forall (m:{m: Natural| True}) (n:{n: Natural| True}), geN m n->geqN m n). 
+Defined.
+Theorem ge_geq: ge_geq_spec.
+Proof.
+  intros m. intros n. destruct m as [m mp ].  destruct n as [n np ]. 
+  induction m as [| m IHm ]. 
+    { destruct n as [ | n ]. smt_now smt_trivial. smt_now smt_trivial. }
+    { destruct n as [ | n ]. smt_now smt_trivial. smt_app IHm. }
+Qed.
+
+Definition mult_zero_spec: Prop. 
+Proof. smt_now unshelve refine (forall (m:{m: Natural| True}) (n:{n: Natural| True}), ((` (m))<>(ZeroN)) /\ ((` (n))<>(ZeroN))->geqN (subsumptionCast Natural (fun VV: Natural => ((` (mult_unrefined m n))=(VV))) (fun m: Natural => True) _ (mult m n)) n). 
+Defined.
+Theorem mult_zero: mult_zero_spec.
+Proof.
+  intros m. intros n. destruct m as [m mp ].  destruct n as [n np ]. 
+  
+    { destruct m as [ | m ]. smt_now smt_trivial. 
+  assertFresh ((` (mult (injectionCast Natural (fun m: Natural => True) (Suc m) _) (injectionCast Natural (fun n: Natural => True) (n) _)))=(` (add (injectionCast Natural (fun m: Natural => True) (n) _) (subsumptionCast Natural (fun VV: Natural => ((` (mult_unrefined (injectionCast Natural (fun m: Natural => True) (m) _) (injectionCast Natural (fun n: Natural => True) (n) _)))=(VV))) (fun n: Natural => True) _ (mult (injectionCast Natural (fun m: Natural => True) (m) _) (injectionCast Natural (fun n: Natural => True) (n) _)))))) as lem using (smt_app (mult_suc_l (injectionCast Natural (fun m: Natural => True) (m) _) (injectionCast Natural (fun n: Natural => True) (n) _)). ). 
+  assertFresh ((` (add (injectionCast Natural (fun m: Natural => True) (n) _) (subsumptionCast Natural (fun VV: Natural => ((` (mult_unrefined (injectionCast Natural (fun m: Natural => True) (m) _) (injectionCast Natural (fun n: Natural => True) (n) _)))=(VV))) (fun n: Natural => True) _ (mult (injectionCast Natural (fun m: Natural => True) (m) _) (injectionCast Natural (fun n: Natural => True) (n) _)))))=(` (add (subsumptionCast Natural (fun VV: Natural => ((` (mult_unrefined (injectionCast Natural (fun m: Natural => True) (m) _) (injectionCast Natural (fun n: Natural => True) (n) _)))=(VV))) (fun m: Natural => True) _ (mult (injectionCast Natural (fun m: Natural => True) (m) _) (injectionCast Natural (fun n: Natural => True) (n) _))) (injectionCast Natural (fun n: Natural => True) (n) _)))) as lem using (smt_app (add_comm (injectionCast Natural (fun m: Natural => True) (n) _) (subsumptionCast Natural (fun VV: Natural => ((` (mult_unrefined (injectionCast Natural (fun m: Natural => True) (m) _) (injectionCast Natural (fun n: Natural => True) (n) _)))=(VV))) (fun n: Natural => True) _ (mult (injectionCast Natural (fun m: Natural => True) (m) _) (injectionCast Natural (fun n: Natural => True) (n) _)))). ). smt_app (ge_zero (injectionCast Natural (fun n: Natural => True) (n) _)). smt_app (add_mono_l (subsumptionCast Natural (fun VV: Natural => ((` (mult_unrefined (injectionCast Natural (fun m: Natural => True) (m) _) (injectionCast Natural (fun n: Natural => True) (n) _)))=(VV))) (fun m: Natural => True) _ (mult (injectionCast Natural (fun m: Natural => True) (m) _) (injectionCast Natural (fun n: Natural => True) (n) _))) (injectionCast Natural (fun n: Natural => True) (n) _)). smt_app (ge_geq (subsumptionCast Natural (fun VV: Natural => ((` (add_unrefined (injectionCast Natural (fun m: Natural => True) (m) _) (injectionCast Natural (fun n: Natural => True) (n) _)))=(VV))) (fun m: Natural => True) _ (add (subsumptionCast Natural (fun VV: Natural => ((` (mult_unrefined (injectionCast Natural (fun m: Natural => True) (m) _) (injectionCast Natural (fun n: Natural => True) (n) _)))=(VV))) (fun m: Natural => True) _ (mult (injectionCast Natural (fun m: Natural => True) (m) _) (injectionCast Natural (fun n: Natural => True) (n) _))) (injectionCast Natural (fun n: Natural => True) (n) _))) (injectionCast Natural (fun n: Natural => True) (n) _)). }
+Qed.
+
+Definition ge_anti_comm_spec: Prop. 
+Proof. smt_now unshelve refine (forall (m:{m: Natural| True}) (n:{n: Natural| True}), geN m n->not(geN n m)). 
+Defined.
+Theorem ge_anti_comm: ge_anti_comm_spec.
+Proof.
+  intros m. intros n. destruct m as [m mp ].  destruct n as [n np ]. 
+  induction m as [| m IHm ]. 
+    { destruct n as [ | n ]. smt_now smt_trivial. smt_now smt_trivial. }
+    { destruct n as [ | n ]. smt_now smt_trivial. smt_app IHm. }
+Qed.
+
+Definition ge_irreflexive_spec: Prop. 
+Proof. smt_now unshelve refine (forall (m:{m: Natural| True}) (n:{n: Natural| True}), geN m n->not(eqN m n)). 
+Defined.
+Theorem ge_irreflexive: ge_irreflexive_spec.
+Proof.
+  intros m. intros n. destruct m as [m mp ].  destruct n as [n np ]. 
+  induction m as [| m IHm ]. 
+    { smt_now smt_trivial. }
+    { destruct n as [ | n ]. smt_now smt_trivial. smt_app IHm. }
+Qed.
+
+Definition ge_trans_spec: Prop. 
+Proof. smt_now unshelve refine (forall (m:{m: Natural| True}) (n:{n: Natural| True}) (o:{o: Natural| True}), geN m n /\ geN n o->geN m o). 
+Defined.
+Theorem ge_trans: ge_trans_spec.
+Proof.
+  intros m. intros n. intros o. destruct m as [m mp ].  destruct n as [n np ].  destruct o as [o op ]. 
+  induction m as [| m IHm ]. 
+    { smt_now smt_trivial. }
+    { destruct m as [ | m ]. smt_now smt_trivial. destruct o as [ | lq_anf7205759403792798641 ]. smt_now smt_trivial. destruct n as [ | n ]. destruct () as [ ]. destruct o as [ | o ]. destruct () as [ ]. smt_app IHm. }
+Qed.
+
+Definition ge_eq_trans_spec: Prop. 
+Proof. smt_now unshelve refine (forall (m:{m: Natural| True}) (n:{n: Natural| True}) (o:{o: Natural| True}), eqN n o /\ geN m n->geN m o). 
+Defined.
+Theorem ge_eq_trans: ge_eq_trans_spec.
+Proof.
+  intros m. intros n. intros o. destruct m as [m mp ].  destruct n as [n np ].  destruct o as [o op ]. 
+  induction m as [| m IHm ]. 
+    { destruct o as [ | ds_d1cb ]. smt_now smt_trivial. smt_now smt_trivial. }
+    { destruct m as [ | m ]. smt_now smt_trivial. destruct o as [ | lq_anf7205759403792798654 ]. smt_now smt_trivial. destruct n as [ | n ]. destruct () as [ ]. destruct o as [ | o ]. destruct () as [ ]. smt_app IHm. }
+Qed.
+
+Definition geq_suc_l_spec: Prop. 
+Proof. smt_now unshelve refine (forall (m:{m: Natural| True}) (n:{n: Natural| geqN m n}), geqN (injectionCast Natural (fun m: Natural => True) (Suc (` (m))) _) (subsumptionCast Natural (fun n: Natural => geqN m n) (fun n: Natural => True) _ (n))). 
+Defined.
+Theorem geq_suc_l: geq_suc_l_spec.
+Proof.
+  intros m. intros n. destruct m as [m mp ].  destruct n as [n np ]. 
+  induction m as [| m IHm ]. 
+    { destruct n as [ | n ]. smt_now smt_trivial. smt_now smt_trivial. }
+    { destruct n as [ | n ]. smt_now smt_trivial. smt_app IHm. }
+Qed.
+
+Definition geq_ge_suc_spec: Prop. 
+Proof. smt_now unshelve refine (forall (m:{m: Natural| True}) (n:{n: Natural| geqN m (subsumptionCast Natural (fun n: Natural => geqN m n) (fun n: Natural => True) I (n))}), geN (injectionCast Natural (fun m: Natural => True) (Suc (` (m))) _) (subsumptionCast Natural (fun n: Natural => geqN m (subsumptionCast Natural (fun n: Natural => geqN m n) (fun n: Natural => True) I (n))) (fun n: Natural => True) _ (n))). 
+Defined.
+Theorem geq_ge_suc: geq_ge_suc_spec.
+Proof.
+  intros m. intros n. destruct m as [m mp ].  destruct n as [n np ]. 
+  induction m as [| m IHm ]. 
+    { destruct n as [ | n ]. smt_now smt_trivial. smt_now smt_trivial. }
+    { destruct n as [ | n ]. smt_now smt_trivial. smt_app IHm. }
+Qed.
+
+Definition ge_suc_l_spec: Prop. 
+Proof. smt_now unshelve refine (forall (m:{m: Natural| True}) (n:{n: Natural| geN m (subsumptionCast Natural (fun n: Natural => geqN m (subsumptionCast Natural (fun n: Natural => geqN m n) (fun n: Natural => True) I (n))) (fun n: Natural => True) I (n))}), geN (injectionCast Natural (fun m: Natural => True) (Suc (` (m))) _) (subsumptionCast Natural (fun n: Natural => geN m (subsumptionCast Natural (fun n: Natural => geqN m (subsumptionCast Natural (fun n: Natural => geqN m n) (fun n: Natural => True) I (n))) (fun n: Natural => True) I (n))) (fun n: Natural => True) _ (n))). 
+Defined.
+Theorem ge_suc_l: ge_suc_l_spec.
+Proof.
+  intros m. intros n. destruct m as [m mp ].  destruct n as [n np ]. 
+  induction m as [| m IHm ]. 
+    { destruct n as [ | n ]. smt_now smt_trivial. smt_now smt_trivial. }
+    { destruct n as [ | n ]. smt_now smt_trivial. smt_app IHm. }
+Qed.
+
+Definition geq_ge_eq_spec: Prop. 
+Proof. smt_now unshelve refine (forall (m:{m: Natural| True}) (n:{n: Natural| True}), ((` (geqN m n))=(geN m n \/ eqN m n))). 
+Defined.
+Theorem geq_ge_eq: geq_ge_eq_spec.
+Proof.
+  intros m. intros n. destruct m as [m mp ].  destruct n as [n np ]. 
+  induction m as [| m IHm ]. 
+    { destruct n as [ | n ]. smt_now smt_trivial. smt_now smt_trivial. }
+    { destruct n as [ | n ]. smt_now smt_trivial. smt_app IHm. }
+Qed.
+
+Definition geq_not_le_spec: Prop. 
+Proof. smt_now unshelve refine (forall (m:{m: Natural| True}) (n:{n: Natural| True}), ((` (geqN m n))=(not(leN m n)))). 
+Defined.
+Theorem geq_not_le: geq_not_le_spec.
+Proof.
+  intros m. intros n. destruct m as [m mp ].  destruct n as [n np ]. 
+  induction m as [| m IHm ]. 
+    { destruct n as [ | n ]. smt_now smt_trivial. smt_now smt_trivial. }
+    { destruct n as [ | n ]. smt_now smt_trivial. smt_app IHm. }
+Qed.
+
+Definition ge_eq_le_exhaustive_spec: Prop. 
+Proof. smt_now unshelve refine (forall (m:{m: Natural| True}) (n:{n: Natural| True}), geN m n \/ eqN m n \/ leN m n). 
+Defined.
+Theorem ge_eq_le_exhaustive: ge_eq_le_exhaustive_spec.
+Proof.
+  intros m. intros n. destruct m as [m mp ].  destruct n as [n np ]. 
+  induction m as [| m IHm ]. 
+    { destruct n as [ | n ]. smt_now smt_trivial. smt_now smt_trivial. }
+    { destruct n as [ | n ]. smt_now smt_trivial. smt_app IHm. }
+Qed.
+
+Definition subt_self_spec: Prop. 
+Proof. smt_now unshelve refine (forall (m:{m: Natural| True}) (n:{n: Natural| True}), eqN m n->((` (subt m (subsumptionCast Natural (fun n: Natural => True) (fun n: Natural => geqN m n) _ (n))))=(ZeroN))). 
+Defined.
+Theorem subt_self: subt_self_spec.
+Proof.
+  intros m. intros n. destruct m as [m mp ].  destruct n as [n np ]. 
+  induction m as [| m IHm ]. 
+    { smt_now smt_trivial. }
+    { destruct n as [ | n ]. smt_now smt_trivial. smt_app IHm. }
+Qed.
+
+Definition subt_suc_l_spec: Prop. 
+Proof. smt_now unshelve refine (forall (m:{m: Natural| True}) (n:{n: Natural| geqN m n}), ((` (subt (injectionCast Natural (fun m: Natural => True) (Suc (` (m))) _) n))=(Suc (` (subt m n))))). 
+Defined.
+Theorem subt_suc_l: subt_suc_l_spec.
+Proof.
+  intros m. intros n. destruct m as [m mp ].  destruct n as [n np ]. 
+  induction m as [| m IHm ]. 
+    { destruct n as [ | lq_anf7205759403792798689 ]. smt_now smt_trivial. destruct () as [ ]. }
+    { destruct n as [ | n ]. smt_now smt_trivial. smt_app IHm. }
+Qed.
+
+Definition geq_suc_spec: Prop. 
+Proof. smt_now unshelve refine (forall (n:{n: Natural| True}), geqN (injectionCast Natural (fun m: Natural => True) (Suc (` (n))) _) n). 
+Defined.
+Theorem geq_suc: geq_suc_spec.
+Proof.
+  intros n. destruct n as [n np ]. 
+  induction n as [| n IHn ]. 
+    { smt_now smt_trivial. }
+    { smt_app IHn. }
+Qed.
+
+Definition subt_leq_spec: Prop. 
+Proof. smt_now unshelve refine (forall (m:{m: Natural| True}) (n:{n: Natural| geqN (injectionCast Natural (fun m: Natural => True) (m) I) n}), geqN m (subsumptionCast Natural (fun o: Natural => ((` (subt_unrefined m n))=(o))) (fun n: Natural => True) _ (subt m (subsumptionCast Natural (fun n: Natural => geqN (injectionCast Natural (fun m: Natural => True) (m) I) n) (fun n: Natural => geqN m n) _ (n))))). 
+Defined.
+Theorem subt_leq: subt_leq_spec.
+Proof.
+  intros m. intros n. destruct m as [m mp ].  destruct n as [n np ]. 
+  induction m as [| m IHm ]. 
+    { destruct n as [ | lq_anf7205759403792798697 ]. smt_now smt_trivial. destruct () as [ ]. }
+    { destruct n as [ | n ]. smt_app (geq_refl (injectionCast Natural (fun n: Natural => True) (m) _)). smt_app IHm. smt_app (geq_suc (injectionCast Natural (fun n: Natural => True) (m) _)). smt_app (geq_trans (injectionCast Natural (fun m: Natural => True) (Suc m) _) (injectionCast Natural (fun n: Natural => True) (m) _) (subsumptionCast Natural (fun o: Natural => ((` (subt_unrefined (injectionCast Natural (fun m: Natural => True) (m) _) (injectionCast Natural (fun n: Natural => geqN (injectionCast Natural (fun m: Natural => True) (m) _) (injectionCast Natural (fun n: Natural => True) (n) _)) (n) _)))=(o))) (fun o: Natural => True) _ (subt (injectionCast Natural (fun m: Natural => True) (m) _) (injectionCast Natural (fun n: Natural => geqN (injectionCast Natural (fun m: Natural => True) (m) _) (injectionCast Natural (fun n: Natural => True) (n) _)) (n) _)))). }
+Qed.
+
+Definition subt_le_spec: Prop. 
+Proof. smt_now unshelve refine (forall (m:{m: Natural| True}) (n:{n: Natural| geqN m (subsumptionCast Natural (fun n: Natural => geqN (injectionCast Natural (fun m: Natural => True) (m) I) n) (fun n: Natural => True) I (n))}), ((` (n))<>(ZeroN))->geN m (subsumptionCast Natural (fun o: Natural => ((` (subt_unrefined m n))=(o))) (fun n: Natural => True) _ (subt m (subsumptionCast Natural (fun n: Natural => geqN m (subsumptionCast Natural (fun n: Natural => geqN (injectionCast Natural (fun m: Natural => True) (m) I) n) (fun n: Natural => True) I (n))) (fun n: Natural => geqN m n) _ (n))))). 
+Defined.
+Theorem subt_le: subt_le_spec.
+Proof.
+  intros m. intros n. destruct m as [m mp ].  destruct n as [n np ]. 
+  
+    { destruct m as [ | m ]. destruct n as [ | lq_anf7205759403792798710 ]. smt_now smt_trivial. destruct () as [ ]. destruct n as [ | n ]. smt_app (geq_refl (injectionCast Natural (fun n: Natural => True) (m) _)). 
+  assertFresh ((` (subt (injectionCast Natural (fun m: Natural => True) (Suc m) _) (injectionCast Natural (fun n: Natural => geqN (injectionCast Natural (fun m: Natural => True) (m) _) (injectionCast Natural (fun n: Natural => True) (n) _)) (Suc n) _)))=(` (subt (injectionCast Natural (fun m: Natural => True) (m) _) (injectionCast Natural (fun n: Natural => geqN (injectionCast Natural (fun m: Natural => True) (m) _) (injectionCast Natural (fun n: Natural => True) (n) _)) (n) _)))) as lem using smt_trivial. . smt_app (subt_leq (injectionCast Natural (fun m: Natural => True) (m) _) (injectionCast Natural (fun n: Natural => geqN (injectionCast Natural (fun m: Natural => True) (injectionCast Natural (fun m: Natural => True) (m) _) I) (injectionCast Natural (fun n: Natural => True) (n) _)) (n) _)). smt_app (geq_ge_suc (injectionCast Natural (fun m: Natural => True) (m) _) (subsumptionCast Natural (fun o: Natural => ((` (subt_unrefined (injectionCast Natural (fun m: Natural => True) (m) _) (injectionCast Natural (fun n: Natural => geqN (injectionCast Natural (fun m: Natural => True) (m) _) (injectionCast Natural (fun n: Natural => True) (n) _)) (n) _)))=(o))) (fun n: Natural => geqN (injectionCast Natural (fun m: Natural => True) (m) _) (subsumptionCast Natural (fun n: Natural => geqN (injectionCast Natural (fun m: Natural => True) (m) _) (injectionCast Natural (fun n: Natural => True) (n) _)) (fun n: Natural => True) I (injectionCast Natural (fun n: Natural => True) (n) _))) _ (subt (injectionCast Natural (fun m: Natural => True) (m) _) (injectionCast Natural (fun n: Natural => geqN (injectionCast Natural (fun m: Natural => True) (m) _) (injectionCast Natural (fun n: Natural => True) (n) _)) (n) _)))). smt_app (eq_equal (subsumptionCast Natural (fun o: Natural => ((` (subt_unrefined (injectionCast Natural (fun m: Natural => True) (m) _) (injectionCast Natural (fun n: Natural => geqN (injectionCast Natural (fun m: Natural => True) (m) _) (injectionCast Natural (fun n: Natural => True) (n) _)) (n) _)))=(o))) (fun m: Natural => True) _ (subt (injectionCast Natural (fun m: Natural => True) (m) _) (injectionCast Natural (fun n: Natural => geqN (injectionCast Natural (fun m: Natural => True) (m) _) (injectionCast Natural (fun n: Natural => True) (n) _)) (n) _))) (subsumptionCast Natural (fun o: Natural => ((` (subt_unrefined (injectionCast Natural (fun m: Natural => True) (m) _) (injectionCast Natural (fun n: Natural => geqN (injectionCast Natural (fun m: Natural => True) (m) _) (injectionCast Natural (fun n: Natural => True) (n) _)) (n) _)))=(o))) (fun n: Natural => True) _ (subt (injectionCast Natural (fun m: Natural => True) (Suc m) _) (injectionCast Natural (fun n: Natural => geqN (injectionCast Natural (fun m: Natural => True) (m) _) (injectionCast Natural (fun n: Natural => True) (n) _)) (Suc n) _)))). smt_app (ge_eq_trans (injectionCast Natural (fun m: Natural => True) (Suc m) _) (subsumptionCast Natural (fun o: Natural => ((` (subt_unrefined (injectionCast Natural (fun m: Natural => True) (m) _) (injectionCast Natural (fun n: Natural => geqN (injectionCast Natural (fun m: Natural => True) (m) _) (injectionCast Natural (fun n: Natural => True) (n) _)) (n) _)))=(o))) (fun n: Natural => True) _ (subt (injectionCast Natural (fun m: Natural => True) (m) _) (injectionCast Natural (fun n: Natural => geqN (injectionCast Natural (fun m: Natural => True) (m) _) (injectionCast Natural (fun n: Natural => True) (n) _)) (n) _))) (subsumptionCast Natural (fun o: Natural => ((` (subt_unrefined (injectionCast Natural (fun m: Natural => True) (m) _) (injectionCast Natural (fun n: Natural => geqN (injectionCast Natural (fun m: Natural => True) (m) _) (injectionCast Natural (fun n: Natural => True) (n) _)) (n) _)))=(o))) (fun o: Natural => True) _ (subt (injectionCast Natural (fun m: Natural => True) (Suc m) _) (injectionCast Natural (fun n: Natural => geqN (injectionCast Natural (fun m: Natural => True) (m) _) (injectionCast Natural (fun n: Natural => True) (n) _)) (Suc n) _)))). }
+Qed.
+
+Definition notZ_spec: Prop. 
+Proof. smt_now unshelve refine (forall (n:{n: Natural| ((` (n))<>(ZeroN))}), geN (injectionCast Natural (fun m: Natural => True) (Suc (` (n))) _) (injectionCast Natural (fun n: Natural => True) (one) _)). 
+Defined.
+Theorem notZ: notZ_spec.
+Proof.
+  intros n. destruct n as [n np ]. 
+  
+    { destruct n as [ | n ]. smt_now smt_trivial. smt_now smt_trivial. }
 Qed.
